confluence proof for case when one is a par step, other is a sec step

examples/wysteria/theory.fst
@@ -1905,4 +1905,50 @@ let pstep_ppar_ppar_confluence #ps pi pi1 pi2 h1 h2 =
     let h23:pstep #ps pi2 (pi13_m, s) = P_par #ps #c1' pi2 p1 hp1 (pi23_m, s) in
     
     IntroR (ExIntro #(protocol ps) #((fun pi3 -> cand (pstep #ps pi1 pi3) (pstep #ps pi2 pi3))) (pi13_m, s) (Conj h13 h23))
+
+val pstep_ppar_psec_confluence:
+  #ps:prins -> pi:protocol ps -> pi1:protocol ps -> pi2:protocol ps
+  -> h1:pstep #ps pi pi1{is_P_par h1} -> h2:pstep #ps pi pi2{is_P_sec h2}
+  -> Tot (cexists #(protocol ps) (fun pi3 -> cand (pstep #ps pi1 pi3) (pstep #ps pi2 pi3)))
+let pstep_ppar_psec_confluence #ps pi pi1 pi2 h1 h2 =
+  let pi_m, s = pi in
+  let pi1_m, s1 = pi1 in
+  let pi2_m, s2 = pi2 in
+  
+  let pi3_m = pi1_m in
+  let s3 = s2 in
+  
+  let h13:pstep #ps pi1 (pi3_m, s3) = P_sec #ps #(P_sec.c' h2) pi1 (P_sec.h h2) (pi3_m, s3) in
+  let h23:pstep #ps pi2 (pi3_m, s3) = P_par #ps #(P_par.c' h1) pi2 (P_par.p h1) (P_par.h h1) (pi3_m, s3) in
+  
+  ExIntro #(protocol ps) #(fun pi3 -> cand (pstep #ps pi1 pi3) (pstep #ps pi2 pi3)) (pi3_m, s3) (Conj h13 h23)
+  
+val pstep_ppar_psec_enter_confluence:
+  #ps:prins -> pi:protocol ps -> pi1:protocol ps -> pi2:protocol ps
+  -> h1:pstep #ps pi pi1{is_P_par h1} -> h2:pstep #ps pi pi2{is_P_sec_enter h2}
+  -> Tot (cexists #(protocol ps) (fun pi3 -> cand (pstep #ps pi1 pi3) (pstep #ps pi2 pi3)))
+let pstep_ppar_psec_enter_confluence #ps pi pi1 pi2 h1 h2 = admit ()
+  
+
+
+
+
+
+
+
+
+
+
+
+
+
+
+
+
+
+
+
+
+
+
   
